feat: dotnet examples (#482)
* feat: dotnet examples

Examples/runtimes/net/src/searchableencryption/VirtualBeaconSearchableEncryptionExample.cs
@@ -1,0 +1,438 @@
+using System;
+using System.Collections.Generic;
+using System.Diagnostics;
+using System.Net;
+using System.Threading;
+using System.Threading.Tasks;
+using Amazon.DynamoDBv2;
+using Amazon.DynamoDBv2.Model;
+using Amazon.KeyManagementService;
+using AWS.Cryptography.DbEncryptionSDK.DynamoDb;
+using AWS.Cryptography.DbEncryptionSDK.DynamoDb.Transforms;
+using AWS.Cryptography.DbEncryptionSDK.StructuredEncryption;
+using AWS.Cryptography.KeyStore;
+using AWS.Cryptography.MaterialProviders;
+
+/*
+  This example demonstrates how to set up a virtual field from two DDB
+  attributes, create a standard beacon with that field, put an item with
+  that beacon, and query against that beacon.
+
+  A virtual field is a field consisting of a transformation of one or more attributes in a DDB item.
+  Virtual fields are useful in querying against encrypted fields that only have a handful of
+  possible values. They allow you to take fields with few possible values, concatenate
+  them to other fields, then query against the combined field. This enables using these types of
+  fields in queries while making it infeasible to identify which beacon values encode
+  the few possible distinct plaintexts. This is explained in more detail below.
+  Virtual fields are not stored in the DDB table. However, they are used to construct
+  a beacon, the value of which is stored.
+
+  For more information on virtual fields, see
+    https://docs.aws.amazon.com/database-encryption-sdk/latest/devguide/beacons.html#virtual-field
+
+  For our example, we will construct a virtual field
+  from two DDB attributes `state` and `hasTestResult` as `state`+prefix(`hasTestResult`, 1).
+  We will then create a beacon out of this virtual field and use it to search.
+
+  This example follows a use case of a database that stores customer test result metadata.
+  Records are indexed by `customer_id` and store a `state` attribute, representing the
+  US state or territory where the customer lives, and a `hasTestResult` boolean attribute,
+  representing whether the customer has a "test result" available. (Maybe this represents
+  some medical test result, and this table stores "result available" metadata.) We assume
+  that values in these fields are uniformly distributed across all possible values for
+  these fields (56 for `state`, 2 for `hasTestResult`), and are uniformly distributed across
+  customer IDs.
+
+  The motivation behind this example is to demonstrate how and why one would use a virtual beacon.
+  In this example, our table stores records with an encrypted boolean `hasTestResult` attribute.
+  We would like to be able to query for customers in a given state with a `true` hasTestResult
+  attribute.
+
+  To be able to execute this query securely and efficiently, we want the following
+  properties on our table:
+   1. Hide the distribution of `hasTestResult` attribute values (i.e. it should be infeasible
+      to determine the percentage of `true`s to `false`s across the dataset from beaconized
+      values)
+   2. Query against a combination of whether `hasTestResult` is true/false and the `state` field
+  We cannot achieve these properties with a standard beacon on a true/false attribute. Following
+  the guidance to choose a beacon length:
+    https://docs.aws.amazon.com/database-encryption-sdk/latest/devguide/choosing-beacon-length.html
+  For a boolean value (in our case, whether `hasTestResult` is true or false), the acceptable
+  bounds for beacon length are either 0 or 1. This corresponds to either not storing a beacon
+  (length 0), or effectively storing another boolean attribute (length 1). With
+  length 0, this beacon is useless for searching (violating property 2); with length 1, this
+  beacon may not hide the attribute (violating property 1).
+  In addition, choosing a longer beacon length does not help us.
+  Each attribute value is mapped to a distinct beacon.
+  Since booleans only have 2 possible attribute values, we will still only have 2 possible
+  beacon values, though those values may be longer. A longer beacon provides no advantages over
+  beacon of length 1 in this situation.
+
+  A compound beacon also does not help.
+  To (over)simplify, a compound beacon is a concatenation of standard beacons,
+  i.e. beacon(`state`)+beacon(`hasTestResult`).
+  The `hasTestResult` beacon is still visible, so we would still have the problems above.
+
+  To achieve these properties, we instead construct a virtual field and use that in our beacon,
+  i.e. beacon(`state`+`hasTestResult`). Assuming these fields are well-distributed across
+  customer IDs and possible values, this gives us both desired properties; we can query against
+  both attributes while hiding information from the underlying data. This is demonstrated in more
+  detail below.
+
+  Running this example requires access to a DDB table  with the
+  following primary key configuration:
+    - Partition key is named "customer_id" with type (S)
+    - Sort key is named "create_time" with type (S)
+  This table must have a Global Secondary Index (GSI) configured named "stateAndHasTestResult-index":
+    - Partition key is named "aws_dbe_b_stateAndHasTestResult" with type (S)
+
+  In this example for storing customer location data, this schema is utilized for the data:
+   - "customer_id" stores a unique customer identifier
+   - "create_time" stores a Unix timestamp
+   - "state" stores an encrypted 2-letter US state or territory abbreviation
+         (https://www.faa.gov/air_traffic/publications/atpubs/cnt_html/appendix_a.html)
+   - "hasTestResult" is not part of the schema, but is an attribute utilized in this example.
+      It stores a boolean attribute (false/true) indicating whether this customer has a test result
+      available.
+
+  The example requires the following ordered input command line parameters:
+    1. DDB table name for table to put/query data from
+    2. Branch key ID for a branch key that was previously created in your key store. See the
+       CreateKeyStoreKeyExample.
+    2. Branch key wrapping KMS key ARN for the KMS key used to create the branch key
+    3. Branch key DDB table name for the DDB table representing the branch key store
+ */
+
+public class VirtualBeaconSearchableEncryptionExample
+{
+    static readonly String GSI_NAME = "stateAndHasTestResult-index";
+
+    public static async Task PutItemQueryItemWithVirtualBeacon(String branchKeyId)
+    {
+        String ddbTableName = TestUtils.SIMPLE_BEACON_TEST_DDB_TABLE_NAME;
+        String branchKeyWrappingKmsKeyArn = TestUtils.TEST_BRANCH_KEY_WRAPPING_KMS_KEY_ARN;
+        String branchKeyDdbTableName = TestUtils.TEST_BRANCH_KEYSTORE_DDB_TABLE_NAME;
+
+        // 1. Construct a length-1 prefix virtual transform.
+        //    `hasTestResult` is a binary attribute, containing either `true` or `false`.
+        //    As an example to demonstrate virtual transforms, we will truncate the value
+        //    of `hasTestResult` in the virtual field to the length-1 prefix of the binary value, i.e.:
+        //     - "true" -> "t"
+        //     - "false -> "f"
+        //    This is not necessary. This is done as a demonstration of virtual transforms.
+        //    Virtual transform operations treat all attributes as strings
+        //    (i.e. the boolean value `true` is interpreted as a string "true"),
+        //    so its length-1 prefix is just "t".
+        var length1PrefixVirtualTransformList = new List<VirtualTransform>();
+        var length1PrefixVirtualTransform = new VirtualTransform
+        {
+            Prefix = new GetPrefix { Length = 1 }
+        };
+        length1PrefixVirtualTransformList.Add(length1PrefixVirtualTransform);
+
+        // 2. Construct the VirtualParts required for the VirtualField
+        var hasTestResultPart = new VirtualPart
+        {
+            Loc = "hasTestResult",
+            // Here, we apply the length-1 prefix virtual transform
+            Trans = length1PrefixVirtualTransformList
+        };
+
+        var statePart = new VirtualPart { Loc = "state" };
+        // Note that we do not apply any transform to the `state` attribute,
+        // and the virtual field will read in the attribute as-is.
+
+        // 3. Construct the VirtualField from the VirtualParts
+        //    Note that the order that virtual parts are added to the virtualPartList
+        //    dictates the order in which they are concatenated to build the virtual field.
+        //    You must add virtual parts in the same order on write as you do on read.
+        var virtualPartList = new List<VirtualPart> { statePart, hasTestResultPart };
+
+        var stateAndHasTestResultField = new VirtualField
+        {
+            Name = "stateAndHasTestResult",
+            Parts = virtualPartList
+        };
+
+        var virtualFieldList = new List<VirtualField> { stateAndHasTestResultField };
+
+        // 4. Configure our beacon.
+        //    The virtual field is assumed to hold a US 2-letter state abbreviation
+        //    (56 possible values = 50 states + 6 territories) concatenated with a binary attribute
+        //    (2 possible values: true/false hasTestResult field), we expect a population size of
+        //    56 * 2 = 112 possible values.
+        //    We will also assume that these values are reasonably well-distributed across
+        //    customer IDs. In practice, this will not be true. We would expect
+        //    more populous states to appear more frequently in the database.
+        //    A more complex analysis would show that a stricter upper bound
+        //    is necessary to account for this by hiding information from the
+        //    underlying distribution.
+        //
+        //    This link provides guidance for choosing a beacon length:
+        //       https://docs.aws.amazon.com/database-encryption-sdk/latest/devguide/choosing-beacon-length.html
+        //    We follow the guidance in the link above to determine reasonable bounds for beacon length:
+        //     - min: log(sqrt(112))/log(2) ~= 3.4, round down to 3
+        //     - max: log((112/2))/log(2) ~= 5.8, round up to 6
+        //    You will somehow need to round results to a nearby integer.
+        //    We choose to round to the nearest integer; you might consider a different rounding approach.
+        //    Rounding up will return fewer expected "false positives" in queries,
+        //       leading to fewer decrypt calls and better performance,
+        //       but it is easier to identify which beacon values encode distinct plaintexts.
+        //    Rounding down will return more expected "false positives" in queries,
+        //       leading to more decrypt calls and worse performance,
+        //       but it is harder to identify which beacon values encode distinct plaintexts.
+        //    We can choose a beacon length between 3 and 6:
+        //     - Closer to 3, we expect more "false positives" to be returned,
+        //       making it harder to identify which beacon values encode distinct plaintexts,
+        //       but leading to more decrypt calls and worse performance
+        //     - Closer to 6, we expect fewer "false positives" returned in queries,
+        //       leading to fewer decrypt calls and better performance,
+        //       but it is easier to identify which beacon values encode distinct plaintexts.
+        //    As an example, we will choose 5.
+        //    Values stored in aws_dbe_b_stateAndHasTestResult will be 5 bits long (0x00 - 0x1f)
+        //    There will be 2^5 = 32 possible HMAC values.
+        //    With a well-distributed dataset (112 values), for a particular beacon we expect
+        //    (112/32) = 3.5 combinations of abbreviation + true/false attribute
+        //    sharing that beacon value.
+        var standardBeaconList = new List<StandardBeacon>();
+        var stateAndHasTestResultBeacon = new StandardBeacon
+        {
+            // This name is the same as our virtual field's name above
+            Name = "stateAndHasTestResult",
+            Length = 5
+        };
+        standardBeaconList.Add(stateAndHasTestResultBeacon);
+
+        // 5. Configure Keystore.
+        //    This example expects that you have already set up a KeyStore with a single branch key.
+        //    See the "CreateKeyStoreTableExample" and "CreateKeyStoreKeyExample" files for how to do this.
+        //    After you create a branch key, you should persist its ID for use in this example.
+        var keyStore = new KeyStore(new KeyStoreConfig
+        {
+            KmsClient = new AmazonKeyManagementServiceClient(),
+            DdbClient = new AmazonDynamoDBClient(),
+            DdbTableName = branchKeyDdbTableName,
+            LogicalKeyStoreName = branchKeyDdbTableName,
+            KmsConfiguration = new KMSConfiguration { KmsKeyArn = branchKeyWrappingKmsKeyArn }
+        });
+
+        // 6. Create BeaconVersion.
+        //    The BeaconVersion inside the list holds the list of beacons on the table.
+        //    The BeaconVersion also stores information about the keystore.
+        //    BeaconVersion must be provided:
+        //      - keyStore: The keystore configured in the previous step.
+        //      - keySource: A configuration for the key source.
+        //        For simple use cases, we can configure a 'singleKeySource' which
+        //        statically configures a single beaconKey. That is the approach this example takes.
+        //        For use cases where you want to use different beacon keys depending on the data
+        //        (for example if your table holds data for multiple tenants, and you want to use
+        //        a different beacon key per tenant), look into configuring a MultiKeyStore:
+        //          https://docs.aws.amazon.com/database-encryption-sdk/latest/devguide/searchable-encryption-multitenant.html
+        //    We also provide our standard beacon list and virtual fields here.
+        var beaconVersions = new List<BeaconVersion>
+        {
+            new BeaconVersion
+            {
+                VirtualFields = virtualFieldList,
+                StandardBeacons = standardBeaconList,
+                Version = 1, // MUST be 1
+                KeyStore = keyStore,
+                KeySource = new BeaconKeySource
+                {
+                    Single = new SingleKeyStore
+                    {
+                        // `keyId` references a beacon key.
+                        // For every branch key we create in the keystore,
+                        // we also create a beacon key.
+                        // This beacon key is not the same as the branch key,
+                        // but is created with the same ID as the branch key.
+                        KeyId = branchKeyId,
+                        CacheTTL = 6000
+                    }
+                }
+            }
+        };
+
+        // 7. Create a Hierarchical Keyring
+        //    This is a KMS keyring that utilizes the keystore table.
+        //    This config defines how items are encrypted and decrypted.
+        //    NOTE: You should configure this to use the same keystore as your search config.
+        var matProv = new MaterialProviders(new MaterialProvidersConfig());
+        var keyringInput = new CreateAwsKmsHierarchicalKeyringInput
+        {
+            BranchKeyId = branchKeyId,
+            KeyStore = keyStore,
+            TtlSeconds = 6000L
+        };
+        var kmsKeyring = matProv.CreateAwsKmsHierarchicalKeyring(keyringInput);
+
+        // 8. Configure which attributes are encrypted and/or signed when writing new items.
+        //    For each attribute that may exist on the items we plan to write to our DynamoDbTable,
+        //    we must explicitly configure how they should be treated during item encryption:
+        //      - ENCRYPT_AND_SIGN: The attribute is encrypted and included in the signature
+        //      - SIGN_ONLY: The attribute not encrypted, but is still included in the signature
+        //      - DO_NOTHING: The attribute is not encrypted and not included in the signature
+        //    Any attributes that will be used in beacons must be configured as ENCRYPT_AND_SIGN.
+        var attributeActionsOnEncrypt = new Dictionary<String, CryptoAction>
+        {
+            ["customer_id"] = CryptoAction.SIGN_ONLY, // Our partition attribute must be SIGN_ONLY
+            ["create_time"] = CryptoAction.SIGN_ONLY, // Our sort attribute must be SIGN_ONLY
+            ["state"] = CryptoAction.ENCRYPT_AND_SIGN, // Beaconized attributes must be encrypted
+            ["hasTestResult"] = CryptoAction.ENCRYPT_AND_SIGN // Beaconized attributes must be encrypted
+        };
+        // 9. Create the DynamoDb Encryption configuration for the table we will be writing to.
+        //    The beaconVersions are added to the search configuration.
+        var tableConfigs = new Dictionary<String, DynamoDbTableEncryptionConfig>();
+        var config = new DynamoDbTableEncryptionConfig
+        {
+            LogicalTableName = ddbTableName,
+            PartitionKeyName = "customer_id",
+            SortKeyName = "create_time",
+            AttributeActionsOnEncrypt = attributeActionsOnEncrypt,
+            Keyring = kmsKeyring,
+            Search = new SearchConfig
+            {
+                WriteVersion = 1, // MUST be 1
+                Versions = beaconVersions
+            }
+        };
+        tableConfigs.Add(ddbTableName, config);
+
+        // 10. Create config
+        var encryptionConfig = new DynamoDbTablesEncryptionConfig
+        {
+            TableEncryptionConfigs = tableConfigs
+        };
+
+        // 11. Create test items
+
+        // Create item with hasTestResult=true
+        var itemWithHasTestResult = new Dictionary<String, AttributeValue>
+        {
+            ["customer_id"] = new AttributeValue("ABC-123"),
+            ["create_time"] = new AttributeValue { N = "1681495205" },
+            ["state"] = new AttributeValue("CA"),
+            ["hasTestResult"] = new AttributeValue { BOOL = true }
+        };
+
+        // Create item with hasTestResult=false
+        var itemWithNoHasTestResult = new Dictionary<String, AttributeValue>
+        {
+            ["customer_id"] = new AttributeValue("DEF-456"),
+            ["create_time"] = new AttributeValue { N = "1681495205" },
+            ["state"] = new AttributeValue("CA"),
+            ["hasTestResult"] = new AttributeValue { BOOL = false }
+        };
+
+        // 12. If developing or debugging, verify config by checking virtual field values directly
+        var trans = new DynamoDbEncryptionTransforms(encryptionConfig);
+
+        var resolveInput = new ResolveAttributesInput
+        {
+            TableName = ddbTableName,
+            Item = itemWithHasTestResult,
+            Version = 1
+        };
+        var resolveOutput = trans.ResolveAttributes(resolveInput);
+
+        // CompoundBeacons is empty because we have no Compound Beacons configured
+        Debug.Assert(resolveOutput.CompoundBeacons.Count == 0);
+
+        // Verify that VirtualFields has the expected value
+        Debug.Assert(resolveOutput.VirtualFields.Count == 1);
+        Debug.Assert(resolveOutput.VirtualFields["stateAndHasTestResult"] == "CAt");
+
+        // 13. Create a new AWS SDK DynamoDb client using the DynamoDb Encryption Interceptor above
+        var ddb = new Client.DynamoDbClient(trans);
+
+        // 14. Put two items into our table using the above client.
+        //     The two items will differ only in their `customer_id` attribute (primary key)
+        //         and their `hasTestResult` attribute.
+        //     We will query against these items to demonstrate how to use our setup above
+        //         to query against our `stateAndHasTestResult` beacon.
+        //     Before the item gets sent to DynamoDb, it will be encrypted
+        //         client-side, according to our configuration.
+        //     Since our configuration includes a beacon on a virtual field named
+        //         `stateAndHasTestResult`, the client will add an attribute
+        //         to the item with name `aws_dbe_b_stateAndHasTestResult`.
+        //         Its value will be an HMAC truncated to as many bits as the
+        //         beacon's `length` parameter; i.e. 5.
+
+        var itemWithHasTestResultPutRequest = new PutItemRequest
+        {
+            TableName = ddbTableName,
+            Item = itemWithHasTestResult
+        };
+
+        var itemWithHasTestResultPutResponse = await ddb.PutItemAsync(itemWithHasTestResultPutRequest);
+        // Assert PutItem was successful
+        Debug.Assert(itemWithHasTestResultPutResponse.HttpStatusCode == HttpStatusCode.OK);
+
+        var itemWithNoHasTestResultPutRequest = new PutItemRequest
+        {
+            TableName = ddbTableName,
+            Item = itemWithNoHasTestResult
+        };
+
+        var itemWithNoHasTestResultPutResponse = await ddb.PutItemAsync(itemWithNoHasTestResultPutRequest);
+        // Assert PutItem was successful
+        Debug.Assert(itemWithNoHasTestResultPutResponse.HttpStatusCode == HttpStatusCode.OK);
+
+        // 15. Query by stateAndHasTestResult attribute.
+        //     Note that we are constructing the query as if we were querying on plaintext values.
+        //     However, the DDB encryption client will detect that this attribute name has a beacon configured.
+        //     The client will add the beaconized attribute name and attribute value to the query,
+        //         and transform the query to use the beaconized name and value.
+        //     Internally, the client will query for and receive all items with a matching HMAC value in the beacon field.
+        //     This may include a number of "false positives" with different ciphertext, but the same truncated HMAC.
+        //     e.g. if truncate(HMAC("CAt"), 5) == truncate(HMAC("DCf"), 5), the query will return both items.
+        //     The client will decrypt all returned items to determine which ones have the expected attribute values,
+        //         and only surface items with the correct plaintext to the user.
+        //     This procedure is internal to the client and is abstracted away from the user;
+        //     e.g. the user will only see "CAt" and never "DCf", though the actual query returned both.
+        var expressionAttributeValues = new Dictionary<String, AttributeValue>
+        {
+            // We are querying for the item with `state`="CA" and `hasTestResult`=`true`.
+            // Since we added virtual parts as `state` then `hasTestResult`,
+            //     we must write our query expression in the same order.
+            // We constructed our virtual field as `state`+`hasTestResult`,
+            //     so we add the two parts in that order.
+            // Since we also created a virtual transform that truncated `hasTestResult`
+            //     to its length-1 prefix, i.e. "true" -> "t",
+            //     we write that field as its length-1 prefix in the query.
+            [":stateAndHasTestResult"] = new AttributeValue("CAt")
+        };
+
+        var queryRequest = new QueryRequest
+        {
+            TableName = ddbTableName,
+            IndexName = GSI_NAME,
+            KeyConditionExpression = "stateAndHasTestResult = :stateAndHasTestResult",
+            ExpressionAttributeValues = expressionAttributeValues
+        };
+
+        // GSIs are sometimes a little bit behind, so we sleep if the query comes up empty
+        for (int i = 0; i < 10; ++i)
+        {
+            var queryResponse = await ddb.QueryAsync(queryRequest);
+            // Validate query was returned successfully
+            Debug.Assert(queryResponse.HttpStatusCode == HttpStatusCode.OK);
+
+            var attributeValues = queryResponse.Items;
+            // if no results, sleep and try again
+            if (attributeValues.Count == 0)
+            {
+                Thread.Sleep(20);
+                continue;
+            }
+
+            // Validate only 1 item was returned: the item with the expected attributes
+            Debug.Assert(attributeValues.Count == 1);
+            var returnedItem = attributeValues[0];
+            // Validate the item has the expected attributes
+            Debug.Assert(returnedItem["state"].S.Equals("CA"));
+            Debug.Assert(returnedItem["hasTestResult"].BOOL.Equals(true));
+            break;
+        }
+    }
+}
