DynamoDbEncryption/dafny/DynamoDbEncryptionTransforms/src/DeleteItemTransform.dfy
@@ -25,7 +25,7 @@ module DeleteItemTransform {
       //= type=implication
       //# The DeleteItem request MUST NOT refer to any legacy parameters,
       //# specifically Expected and ConditionalOperator MUST NOT be set.
-      && input.sdkInput.Expected.None?
+      && NoMap(input.sdkInput.Expected)
       && input.sdkInput.ConditionalOperator.None?
 
       //= specification/dynamodb-encryption-client/ddb-sdk-integration.md#validate-before-deleteitem
@@ -52,7 +52,7 @@ module DeleteItemTransform {
 
   {
     if input.sdkInput.TableName in config.tableEncryptionConfigs {
-      :- Need(input.sdkInput.Expected.None?, E("Legacy parameter 'Expected' not supported in UpdateItem with Encryption"));
+      :- Need(NoMap(input.sdkInput.Expected), E("Legacy parameter 'Expected' not supported in UpdateItem with Encryption"));
       :- Need(input.sdkInput.ConditionalOperator.None?, E("Legacy parameter 'ConditionalOperator' not supported in UpdateItem with Encryption"));
 
       var tableConfig := config.tableEncryptionConfigs[input.sdkInput.TableName];
@@ -84,7 +84,7 @@ module DeleteItemTransform {
     ensures (
       && output.Success?
       && input.originalInput.TableName in config.tableEncryptionConfigs
-      && input.sdkOutput.Attributes.Some?
+      && !NoMap(input.sdkOutput.Attributes)
     ) ==>
       && var tableConfig := config.tableEncryptionConfigs[input.originalInput.TableName];
       && var oldHistory := old(tableConfig.itemEncryptor.History.DecryptItem);
@@ -129,7 +129,7 @@ module DeleteItemTransform {
     modifies ModifiesConfig(config)
   {
     var tableName := input.originalInput.TableName;
-    if tableName !in config.tableEncryptionConfigs || input.sdkOutput.Attributes.None?
+    if tableName !in config.tableEncryptionConfigs || NoMap(input.sdkOutput.Attributes)
       {
       return Success(DeleteItemOutputTransformOutput(transformedOutput := input.sdkOutput));
     }
